PREFIX : <https://linked.data.gov.au/def/exem/>
PREFIX dcam: <http://purl.org/dc/dcam/>
PREFIX dcterms: <http://purl.org/dc/terms/>
PREFIX foaf: <http://xmlns.com/foaf/0.1/>
PREFIX ont: <https://linked.data.gov.au/def/exem>
PREFIX owl: <http://www.w3.org/2002/07/owl#>
PREFIX prof: <http://www.w3.org/ns/dx/prof/>
PREFIX rdf: <http://www.w3.org/1999/02/22-rdf-syntax-ns#>
PREFIX rdfs: <http://www.w3.org/2000/01/rdf-schema#>
PREFIX sdo: <https://schema.org/>
PREFIX skos: <http://www.w3.org/2004/02/skos/core#>
PREFIX vann: <http://purl.org/vocab/vann/>
PREFIX xsd: <http://www.w3.org/2001/XMLSchema#>

ont:
    a owl:Ontology ;
    sdo:dateCreated "2021-09-28"^^xsd:date ;
    dcterms:creator <http://orcid.org/0000-0002-8742-7730> ;
    sdo:codeRepository "https://github.com/Kurrawong/exem-ont"^^xsd:anyURI ;
    sdo:copyrightHolder <https://kurrawong.ai> ;
    skos:definition "An ontology for the description of examples."@en ;
    sdo:dateModified "2023-06-21"^^xsd:date ;
    sdo:dateIssued "2023-06-21"^^xsd:date ;
    sdo:license
        # <https://rdflicense.linkeddata.es/rdflicense/cc-by4.0> ,
        "https://creativecommons.org/licenses/by/4.0/"^^xsd:anyURI ;
    sdo:publisher <https://kurrawong.ai> ;
    skos:prefLabel "Exemplification Ontology"@en ;
    vann:preferredNamespacePrefix "exem" ;
    owl:versionIRI :0.2 ;
    owl:versionInfo "0.2"@en ;
    skos:historyNote "This ontology was initially created in 2021 and mostly implemented in 2023 for Australian government data modelling projects that wanted to include examples within the models (ontologies)" ;
.

<https://kurrawong.ai>
    a sdo:Organization ;
    sdo:name "KurrawongAI" ;
    sdo:url "https://kurrawong.ai"^^xsd:anyURI ;
.

<http://orcid.org/0000-0002-8742-7730>
    a sdo:Person ;
    sdo:email "nick@kurrawong.ai"^^xsd:anyURI ;
    sdo:memberOf <https://kurrawong.ai> ;
    sdo:name "Nicholas J. Car" ;
.

dcterms:conformsTo
    a owl:ObjectProperty ;
    dcam:rangeIncludes dcterms:Standard ;
    rdfs:isDefinedBy dcterms: ;
    skos:historyNote "Included here as per use in the Profiles Vocabulary" ;
    skos:definition "An established standard to which the described resource conforms"@en ;
    skos:example "See example for :example property" ;
    skos:prefLabel "conforms to"@en ;
    skos:scopeNote "Use this property to indicate if the example itself conforms to a Profile/Standard" ;
.

dcterms:format
    a owl:AnnotationProperty ;
    dcam:rangeIncludes
        dcterms:Extent ,
        dcterms:MediaType ;
    rdfs:isDefinedBy dcterms: ;
    rdfs:range dcterms:MediaTypeOrExtent ;
    skos:example "See example for :example property" ;
    skos:historyNote "Included here as per use in the Profiles Vocabulary" ;
    skos:definition "The file format, physical medium, or dimensions of the resource"@en ;
    skos:prefLabel "format" ;
    skos:scopeNote "Use this property to indicate if the format / Media Type of the example" ;
.

dcterms:source
    a owl:AnnotationProperty ;
    rdfs:isDefinedBy dcterms: ;
    skos:definition "A related resource from which the described resource is derived."@en ;
    skos:example "See example for :example property" ;
    skos:prefLabel "Source"@en ;
    skos:historyNote "Included here as per general metadata use (DCAT, SDO etc.)" ;
    skos:scopeNote """Use this property to indicate a non-RDF resource, such as a web page, from wich this example was derived. Use prov:wasDerivedFrom to indicate an RDF resource. Use skos:historyNote to describe a non-linkable source or to contain a general description of how this example was created.

Use a datatype of xsd:anyURI for web pages""" ;
.

skos:example
    a owl:AnnotationProperty ;
    rdfs:isDefinedBy <http://www.w3.org/2004/02/skos/core> ;
    rdfs:subPropertyOf skos:note ;
    skos:definition "An example of the use of a concept"@en ;
    skos:example """# A simple descriptive example - inline text
    ex:class-x
        a owl:Class ;
        skos:prefLabel "Class X"@en ;
        skos:example "Description of use of Class X" ;
.""" ;
    skos:historyNote "Included here as the basis for all examples modelling" ;
    skos:prefLabel "example"@en ;
    skos:scopeNote "Do not use this property: it is included only to facilitate understanding of the :example property" ;
.

prof:hasArtifact
    a owl:ObjectProperty ;
    rdfs:domain prof:ResourceDescriptor ;
    rdfs:isDefinedBy prof: ;
    skos:example "See the use for :example. If the resource was remote, rather than a local literal value, this property could be used instead of rdf:value" ;
    skos:historyNote "Included here as per use in the Profiles Vocabulary" ;
    skos:definition "The URL of a downloadable file with particulars such as its format and role indicated by the Resource Descriptor"@en ;
    skos:prefLabel "has artifact"@en ;
    skos:scopeNote "Use this property to indicate a remote object that contains the example's content" ;
.

prof:hasRole
    a owl:ObjectProperty ;
    rdfs:domain prof:ResourceDescriptor ;
    rdfs:isDefinedBy prof: ;
    rdfs:range skos:Concept ;
    skos:example "See example for :example property" ;
    skos:historyNote "Included here as per use in the Profiles Vocabulary" ;
    skos:definition "The function of an artifact described by a Resource Descriptor, such as specification, guidance etc."@en ;
    skos:prefLabel "has role"@en ;
    skos:scopeNote "Use this property to indicate what role the example plays with respect to the thing being exemplified" ;
.

foaf:depiction
    a owl:ObjectProperty ;
    rdfs:domain owl:Thing ;
    rdfs:isDefinedBy foaf: ;
    rdfs:range xsd:anyURI ;
    rdfs:subPropertyOf rdfs:value ;
    owl:inverseOf foaf:depicts ;
    skos:definition "A depiction of some thing"@en ;
    skos:example """# an example of using foaf:depiction to link to an image
# for the imaginary property ex:hasNumberOfLegs
PREFIX : <https://linked.data.gov.au/def/exem/>
PREFIX dcterms: <http://purl.org/dc/terms/>
PREFIX ex: <http://example.com/>
PREFIX foaf: <http://xmlns.com/foaf/0.1/>
PREFIX prof: <http://www.w3.org/ns/dx/prof/>
PREFIX rdf: <http://www.w3.org/1999/02/22-rdf-syntax-ns#>
PREFIX sdo: <https://schema.org/>

ex:hasNumberOfLegs
    a rdf:Property ;
    :example [
        sdo:name "Remote image of legs" ;
        foaf:depiction "http://some-image-online.com/img/milli" ;
        dcterms:format "image/png" ;
    ] ;
.""" ;
    skos:historyNote "Included here to indicate images" ;
    skos:prefLabel "depiction" ;
    skos:scopeNote "Use this property to indicate an image that is the content of the example. The image must be available at a URL" ;
.

prof:ResourceDescriptor
    a owl:Class ;
    rdfs:isDefinedBy prof: ;
    skos:definition "A description of a resource that defines an aspect - a particular part, feature or role - of a Profile"@en ;
    skos:example "See example for :example property" ;
    skos:historyNote "Included here as per use in the Profiles Vocabulary" ;
    skos:prefLabel "Resource Descriptor"@en ;
.

:example
    a owl:ObjectProperty ;
    rdfs:ifDefinedBy ont: ;
    rdfs:subPropertyOf skos:example ;
    skos:definition "" ;
    skos:example """# an RDF Turtle example of the use of this property
# for the imaginary property ex:hasNumberOfLegs
PREFIX : <https://linked.data.gov.au/def/exem/>
PREFIX dcterms: <http://purl.org/dc/terms/>
PREFIX egroles: <https://linked.data.gov.au/def/exem/roles/>
PREFIX ex: <http://example.com/>
PREFIX prof: <http://www.w3.org/ns/dx/prof/>
PREFIX rdf: <http://www.w3.org/1999/02/22-rdf-syntax-ns#>
PREFIX sdo: <https://schema.org/>

ex:hasNumberOfLegs
    a rdf:Property ;
    :example [
        a prof:ResourceDescriptor ;
        sdo:name "Simple RDF Example" ;
        rdf:value '''ex:millipede-a
    a ex:Animal ;
    :hasNumberOfLegs 120 ;
.''' ;
        dcterms:format "text/turtle" ;
        prof:hasRole egroles:CanonicalExample ;
    ] ;
.""" ;
    skos:historyNote "Created in this ontology" ;
    skos:prefLabel "example" ;
.

rdf:value
    a rdf:Property ;
    rdf:ifDefinedBy rdf: ;
    skos:definition "Idiomatic property used for structured values" ;
    skos:example "See example for :example property" ;
    skos:historyNote "Included here as the basic way to indicate a literal example value" ;
    skos:prefLabel "value" ;
.
